transformations/Moore2Mealy/MealyWF.v
@@ -1,18 +1,19 @@
 
 Require Import Moore2Mealy.Mealy Moore2Mealy.MealySemantics. 
 Import String.
+Import Id.
 
-Definition unique_names (m:M) := 
+Definition unique_ids (m:M) := 
   forall e1 e2,
   List.In (StateElement e1) m.(Model.modelElements) ->
   List.In (StateElement e2) m.(Model.modelElements) ->
-  e1.(State_name) = e2.(State_name) ->
+  e1.(State_id) = e2.(State_id) ->
   e1 = e2.
 
-(** Two states with the same name are equals because a state only contains a name. *)
-Lemma always_unique_names :
-  forall m, unique_names m.
-  unfold unique_names.
+(** Two states with the same id are equals because a state only contains an id. *)
+Lemma always_unique_ids :
+  forall m, unique_ids m.
+  unfold unique_ids.
   intros m e1 e2 H1 H2 E.
   destruct e1, e2.
   simpl in E.
@@ -20,7 +21,7 @@ Lemma always_unique_names :
 Qed.
 
 (* fixme : generalise-me *)
-Lemma In_1 : forall (m:Mealy.M) e,
+Lemma In_state : forall (m:Mealy.M) e,
          List.In (StateElement e) (Model.modelElements m) <-> List.In e
     (OptionListUtils.lift_list (get_E_data State_K)
        (Model.modelElements m)).
@@ -41,12 +42,12 @@ Qed.
 
 Lemma in_find : (* fixme : use the concept of discriminant proposition for the proof *)
   forall m n e,
-    unique_names m ->
+    unique_ids m ->
     List.In (StateElement e) m.(Model.modelElements) ->
-    e.(State_name) = n ->
+    e.(State_id) = n ->
     OptionListUtils.find_lift 
       (get_E_data State_K)
-      (fun s : State_t => (n =? s.(State_name))%string)
+      (fun s : State_t => (NodeId_beq n  s.(State_id)))
            m.(Model.modelElements) = 
          Some e.
 Proof.
@@ -57,13 +58,13 @@ Proof.
   + f_equal. 
     apply List.find_some in E.
     destruct E as (IN2 & EQ).
-    apply In_1 in IN2.
-    apply String.eqb_eq in EQ. subst. apply H ; auto.
-  + apply List.find_none with (x:= {| State_name := n |}) in E ; [ |  ].
-     apply String.eqb_neq in E.
-     simpl in E.
-     contradiction.
-     apply In_1.  assumption.
+    apply In_state in IN2.
+    apply internal_NodeId_dec_bl in EQ. subst. apply H ; auto.
+  + apply List.find_none with (x:= {| State_id := n |}) in E ; [ |  ].
+    unfold State_id in E.
+     rewrite internal_NodeId_dec_lb in E. discriminate.
+     reflexivity.
+     apply In_state.  assumption.
 Qed.
 
 
