transformations/Moore2Mealy/MooreWF.v
@@ -1,15 +1,16 @@
 
 Require Import Moore2Mealy.Moore Moore2Mealy.MooreSemantics.
 Import String.
+Import Id.
 
-Definition unique_names (m:Moore.M) := 
+Definition unique_ids (m:Moore.M) := 
   forall e1 e2,
     List.In (StateElement e1) m.(Model.modelElements) ->
     List.In (StateElement e2) m.(Model.modelElements) ->
-    e1.(State_name) = e2.(State_name) ->
+    e1.(State_id) = e2.(State_id) ->
     e1 = e2.
 
-Lemma In_1 : forall (m:Moore.M) e,
+Lemma In_state : forall (m:Moore.M) e,
          List.In (StateElement e) (Model.modelElements m) <-> List.In e
     (OptionListUtils.lift_list (get_E_data State_K)
        (Model.modelElements m)).
@@ -23,18 +24,18 @@ Proof.
   {
     apply OptionListUtils.In_lift in H.
     destruct H as (e2 & (G & IN2)).
-    destruct e2 ; [ unfold get_E_data in G ; injection G ; intro ; subst| discriminate G]. 
+    destruct e2 ; [ PropUtils.inj G| discriminate G]. 
     assumption.
   }
 Qed.
 
 Lemma in_find : 
   forall m n e,
-    unique_names m ->
+    unique_ids m ->
     List.In (StateElement e) m.(Model.modelElements) ->
-    e.(State_name) = n ->
+    e.(State_id) = n ->
     OptionListUtils.find_lift (get_E_data State_K)
-           (fun s : State_t => (n =? s.(State_name))%string)
+           (fun s : State_t => (NodeId_beq n  s.(State_id)))
            m.(Model.modelElements) = 
          Some e.
 Proof.
@@ -44,15 +45,15 @@ Proof.
   + 
     apply List.find_some in E.
     destruct E as (IN2 & EQ).
-    apply In_1 in IN2.
+    apply In_state in IN2.
     f_equal.
     apply H ; [ exact IN2 | exact H0 | ].
-    apply String.eqb_eq in EQ.
+    apply internal_NodeId_dec_bl in EQ. 
     congruence.
    + apply List.find_none with (x:= e) in E ; [ |  ].
-     apply String.eqb_neq in E.
-     congruence.
-     apply In_1 ; assumption.
+     rewrite internal_NodeId_dec_lb in E.
+     congruence. congruence.
+     apply In_state ; assumption.
      
 Qed.
 
