transformations/Moore2Mealy/MooreSemantics.v
@@ -5,9 +5,10 @@ Require Import transformations.Moore2Mealy.Moore.
 Require Import core.Model.
 Require Import core.utils.Utils.
 
+Require Import Id.
 
 Definition initialState (m: M) : option State_t :=
-    find_lift (get_E_data State_K) (fun s => eqb "S0" s.(State_name)) m.(modelElements).
+    find_lift (get_E_data State_K) (fun s => NodeId_beq (Id "S0") s.(State_id)) m.(modelElements).
 
 Definition State_outTransitions (m: M) (s: State_t) : list Transition_t :=
     filter_lift 
