transformations/Moore2Mealy/tests/sampleMoore.v
@@ -4,17 +4,23 @@ Require Import String.
 Require Import transformations.Moore2Mealy.Moore.
 Open Scope string_scope.
 
+Import Id.
+
 (* S0("a") --"A"-> S1("b") --"B"-| 
                       /\         |
                        |         |
                        -----------
 *)
 
+
+Definition id0 := Id "S0".
+Definition id1 := Id "S1".
+
 Definition InputModel : Model Moore.MM :=
   let t0 := Build_Transition_t 0 "A" in 
   let t1 := Build_Transition_t 1 "B" in
-  let s0 := Build_State_t "S0" "a" in
-  let s1 := Build_State_t "S1" "b" in
+  let s0 := Build_State_t id0 "a" in
+  let s1 := Build_State_t id1 "b" in
   Build_Model Moore.MM
     (
       (TransitionElement t0) :: 
