transformations/Moore2Mealy/theorems/Elements.v
@@ -1,0 +1,68 @@
+Require Moore2Mealy.MooreSemantics.
+Require Moore2Mealy.MealySemantics.
+Require Moore2Mealy.Moore2Mealy.
+Require Moore2Mealy.MooreWF.
+Require Moore2Mealy.MealyWF.
+
+Import OptionUtils.
+
+Definition convert (s:Moore.State_t) : Mealy.State_t :=
+  {| Mealy.State_id := s.(Moore.State_id) |}.
+
+Definition convert_transition  (m: Moore.M)  (t : Moore.Transition_t)   :option Mealy.Transition_t :=
+  match Moore.getTransition_target m t with
+  | None => None
+  | Some s => Some (Mealy.Build_Transition_t t.(Moore.Transition_id) t.(Moore.Transition_input) s.(Moore.State_output))
+  end.
+
+Lemma convert_transition_ok : forall (m:Moore.M) t,
+    Moore.WF1 m ->
+    List.In (Moore.TransitionElement t) m.(Model.modelElements) -> 
+    SUCCESS (convert_transition m t).
+Proof.
+  intros m t H0 H.
+  apply H0 in H.
+  destruct H as [s H].
+  unfold convert_transition.
+  exists (Mealy.Build_Transition_t t.(Moore.Transition_id) t.(Moore.Transition_input) s.(Moore.State_output)).
+  simpl.
+  destruct t.
+  Tactics.destruct_match.
+  + PropUtils.inj H.
+    reflexivity.
+  + discriminate.
+Qed.  
+
+
+Lemma state_element_fw : 
+  forall (s:Moore.State_t) (m:Moore.M),
+    List.In (Moore.StateElement s) (Model.modelElements m) ->
+    List.In (Mealy.StateElement (convert s))  (Semantics.execute  Moore2Mealy.Moore2Mealy m).(Model.modelElements).
+Proof.
+  intros s m IN.
+  eapply Tactics.in_modelElements_execute_left.
+  + apply Certification.allTuples_incl_length.
+    apply ListUtils.incl_singleton.
+    exact IN.
+    compute ; auto.
+  + apply List.in_eq. (* first rule *)
+  + reflexivity.
+  + compute. left. reflexivity.
+  + apply List.in_eq. 
+  + destruct s.
+    simpl.
+    reflexivity.
+Qed.
+
+Lemma state_element_bw :
+  forall (s:Mealy.State_t) (m:Moore.M),
+    List.In (Mealy.StateElement s) (Model.modelElements (Semantics.execute  Moore2Mealy.Moore2Mealy m)) ->
+    exists s0,
+      List.In (Moore.StateElement s0) (Model.modelElements m) /\ s = convert s0.
+Proof.
+  intros s m H.
+  core.Tactics.exploit_element_in_result H.
+  exists t0.
+  split ; auto.
+Qed.
+
