transformations/Moore2Mealy/theorems/WFStable.v
@@ -1,0 +1,15 @@
+Require Moore2Mealy.MooreSemantics.
+Require Moore2Mealy.MealySemantics.
+Require Moore2Mealy.Moore2Mealy.
+Require Moore2Mealy.MooreWF.
+Require Moore2Mealy.MealyWF.
+Require Moore2Mealy.theorems.Elements.
+
+
+Lemma unique_ids_preserved_fw : forall m,
+    MooreWF.unique_ids m -> 
+    MealyWF.unique_ids (Semantics.execute Moore2Mealy.Moore2Mealy m).
+Proof.
+  intros ; apply MealyWF.always_unique_ids.
+Qed.
+
