transformations/Moore2MealyALT/MealySemantics.v
@@ -66,3 +66,4 @@ Compute execute MealyTest ("A"::"A"::nil). (* None *)
 
 
 
+
